src/ReactorModel/Objects/Reactor/Core.lean
@@ -12,23 +12,16 @@ protected inductive Core
 
 namespace Core
 
-protected def ports : Reactor.Core → ID ⇀ Port             | mk p _ _ _ _ => p
-protected def acts :  Reactor.Core → ID ⇀ Time.Tag ⇀ Value | mk _ a _ _ _ => a
-protected def state : Reactor.Core → ID ⇀ Value            | mk _ _ s _ _ => s 
-protected def rcns :  Reactor.Core → ID ⇀ Reaction         | mk _ _ _ r _ => r
-protected def nest :  Reactor.Core → ID ⇀ Reactor.Core     | mk _ _ _ _ n => n
-
-theorem ext_iff : {rtr₁ rtr₂ : Reactor.Core} → rtr₁ = rtr₂ ↔ 
-    rtr₁.ports = rtr₂.ports ∧ rtr₁.acts = rtr₂.acts ∧ rtr₁.state = rtr₂.state ∧ 
-    rtr₁.rcns = rtr₂.rcns ∧ rtr₁.nest  = rtr₂.nest
-  | mk .., mk .. => by simp_all [Core.ports, Core.state, Core.rcns, Core.acts, Core.nest]
-
 instance : ReactorType Reactor.Core where
-  ports := Reactor.Core.ports
-  acts  := Reactor.Core.acts
-  state := Reactor.Core.state
-  rcns  := Reactor.Core.rcns
-  nest  := Reactor.Core.nest
+  ports | mk p _ _ _ _ => p
+  acts  | mk _ a _ _ _ => a
+  state | mk _ _ s _ _ => s 
+  rcns  | mk _ _ _ r _ => r
+  nest  | mk _ _ _ _ n => n
+
+open ReactorType in 
+instance : ReactorType.Extensional Reactor.Core where
+  ext_iff := by intro (mk ..) (mk ..); simp [ports, state, rcns, acts, nest]
 
 end Core
 end Reactor
