src/ReactorModel/Objects/Reactor/Proper.lean
@@ -4,43 +4,28 @@ import ReactorModel.Objects.Reactor.TypeClasses.Proper
 open ReactorType in
 structure Reactor where
   raw : Reactor.Raw
-  private wf : Wellformed raw
+  wf  : Wellformed raw
 
 namespace Reactor
 
-def ports : Reactor → ID ⇀ Port             := (·.raw.ports)
-def acts  : Reactor → ID ⇀ Time.Tag ⇀ Value := (·.raw.acts)
-def state : Reactor → ID ⇀ Value            := (·.raw.state)
-def rcns  : Reactor → ID ⇀ Reaction         := (·.raw.rcns)
+open ReactorType in
+instance : ReactorType Reactor where
+  ports    := ports ∘ raw
+  acts     := acts  ∘ raw
+  state    := state ∘ raw
+  rcns     := rcns  ∘ raw
+  nest rtr := 
+    nest rtr.raw |>.attach.map fun ⟨raw, h⟩ => { 
+      raw := raw, 
+      wf := rtr.wf.nested h.choose_spec 
+    }
 
-def nest (rtr : Reactor) : ID ⇀ Reactor :=
-  rtr.raw.nest.attach.map fun ⟨raw, h⟩ => { raw := raw, wf := rtr.wf.nested h.choose_spec }
-
-private theorem nest_raw_comm (rtr : Reactor) : 
-    rtr.raw.nest = rtr.nest.map Reactor.raw := by
-  simp [nest, Partial.map_map, Function.comp, Partial.attach_map_val]
-
-private theorem ext_iff_raw : {rtr₁ rtr₂ : Reactor} → (rtr₁ = rtr₂ ↔ rtr₁.raw = rtr₂.raw)
-  | mk .., mk .. => by simp
-
-theorem ext_iff {rtr₁ rtr₂ : Reactor} : 
-    rtr₁ = rtr₂ ↔ 
-    rtr₁.ports = rtr₂.ports ∧ rtr₁.acts = rtr₂.acts ∧ rtr₁.state = rtr₂.state ∧ 
-    rtr₁.rcns = rtr₂.rcns ∧ rtr₁.nest  = rtr₂.nest := by
-  simp [ext_iff_raw, Reactor.Raw.ext_iff, ports, state, rcns, acts, nest_raw_comm]
-  intros
-  exact {
-    mp := Partial.map_inj (by simp [Function.Injective, ext_iff_raw])
-    mpr := by simp_all
-  }
+-- Note: From this we get `ReactorType.Extensional Reactor` and `ReactorType.Indexable Reactor`.
+instance : ReactorType.Extensional.LawfulCoe Reactor Reactor.Raw where
+  coe := Reactor.raw
+  coe_ext_iff := by intro (mk ..) (mk ..); simp
 
 instance : ReactorType.Proper Reactor where
-  ports      := Reactor.ports
-  acts       := Reactor.acts
-  state      := Reactor.state
-  rcns       := Reactor.rcns
-  nest       := Reactor.nest
-  uniqueIDs  := sorry
   wellformed := sorry
 
 noncomputable def scheduledTags (rtr : Reactor) : Set Time.Tag := 
