src/ReactorModel/Objects/Reactor/Raw.lean
@@ -6,48 +6,31 @@ namespace Reactor
 open ReactorType in
 protected structure Raw where
   core : Reactor.Core
-  private coreUniqueIDs : ∀ {cmp i} (l₁ l₂ : Lineage cmp i core), l₁ = l₂ 
+  uniqueIDs : ∀ {cmp i} (l₁ l₂ : Lineage cmp i core), l₁ = l₂ 
 
 namespace Raw
 
-protected def ports : Reactor.Raw → ID ⇀ Port             := (·.core.ports)
-protected def acts  : Reactor.Raw → ID ⇀ Time.Tag ⇀ Value := (·.core.acts)
-protected def state : Reactor.Raw → ID ⇀ Value            := (·.core.state)
-protected def rcns  : Reactor.Raw → ID ⇀ Reaction         := (·.core.rcns)
-
-protected def nest (rtr : Reactor.Raw) : ID ⇀ Reactor.Raw :=
-  rtr.core.nest.attach.map fun ⟨core, h⟩ => {
-    core := core
-    coreUniqueIDs := by
-      intro _ _ l₁ l₂
-      injection rtr.coreUniqueIDs (.nest h.choose_spec l₁) (.nest h.choose_spec l₂)
-  }
-
-private theorem nest_core_comm (rtr : Reactor.Raw) : 
-    rtr.core.nest = rtr.nest.map Raw.core := by
-  simp [Raw.nest, Partial.map_map, Function.comp, Partial.attach_map_val]
-
-private theorem ext_iff_core : {rtr₁ rtr₂ : Reactor.Raw} → (rtr₁ = rtr₂ ↔ rtr₁.core = rtr₂.core)
-  | mk .., mk .. => by simp
-
-theorem ext_iff {rtr₁ rtr₂ : Reactor.Raw} : 
-    rtr₁ = rtr₂ ↔ 
-    rtr₁.ports = rtr₂.ports ∧ rtr₁.acts = rtr₂.acts ∧ rtr₁.state = rtr₂.state ∧ 
-    rtr₁.rcns = rtr₂.rcns ∧ rtr₁.nest  = rtr₂.nest := by
-  simp [ext_iff_core, Reactor.Core.ext_iff, Raw.ports, Raw.state, Raw.rcns, Raw.acts, nest_core_comm]
-  intros
-  exact {
-    mp := Partial.map_inj (by simp [Function.Injective, ext_iff_core])
-    mpr := by simp_all
-  }
+open ReactorType in
+instance : ReactorType Reactor.Raw where
+  ports    := ports ∘ core
+  acts     := acts  ∘ core
+  state    := state ∘ core
+  rcns     := rcns  ∘ core
+  nest rtr := 
+    nest rtr.core |>.attach.map fun ⟨core, h⟩ => {
+      core := core
+      uniqueIDs := by
+        intro _ _ l₁ l₂
+        injection rtr.uniqueIDs (.nest h.choose_spec l₁) (.nest h.choose_spec l₂)
+    }
 
 instance : ReactorType.Indexable Reactor.Raw where
-  ports     := Reactor.Raw.ports
-  acts      := Reactor.Raw.acts
-  state     := Reactor.Raw.state
-  rcns      := Reactor.Raw.rcns
-  nest      := Reactor.Raw.nest
   uniqueIDs := sorry
+
+-- Note: From this we get `ReactorType.Extensional Reactor.Raw`.
+instance : ReactorType.Extensional.LawfulCoe Reactor.Raw Reactor.Core where
+  coe := Reactor.Raw.core
+  coe_ext_iff := by intro (mk ..) (mk ..); simp  
 
 end Raw
 end Reactor
